fix until d_sub_tvar_inv_nested_all_false in prop_subtyping

proof/iu_system/uni/decl/prop_subtyping.v
@@ -65,16 +65,16 @@ Qed.
 
 
 Theorem dsub_unit_all_false: forall E T,
-  E ⊢ dtyp_all T ->
-  E ⊢ dtyp_unit <: dtyp_all T ->
+  E ⊢ typ_all T ->
+  E ⊢ typ_unit <: typ_all T ->
   False.
 Proof.
   intros. dependent induction H0.
 Qed.
 
 Theorem dsub_top_all_false: forall E T,
-  E ⊢ dtyp_all T ->
-  E ⊢ dtyp_top <: dtyp_all T ->
+  E ⊢ typ_all T ->
+  E ⊢ typ_top <: typ_all T ->
   False.
 Proof.
   intros. dependent induction H0.
@@ -82,7 +82,7 @@ Qed.
 
 Theorem dsub_top_fv_false: forall E X T,
   ds_in X T ->
-  E ⊢ dtyp_top <: T ->
+  E ⊢ typ_top <: T ->
   False.
 Proof.
   intros. dependent induction H0; try solve [inversion H; eauto].
@@ -90,31 +90,31 @@ Qed.
 
 Theorem dsub_unit_fv_false: forall E X T,
   ds_in X T ->
-  E ⊢ dtyp_unit <: T ->
+  E ⊢ typ_unit <: T ->
   False.
 Proof.
   intros. dependent induction H0; try solve [inversion H; eauto].
 Qed.
 
 
-Hint Resolve dwf_typ_lc_dtyp : subtyping.
+Hint Resolve d_wf_typ_lc_typ : subtyping.
 Hint Resolve dsub_refl : subtyping.
 Hint Resolve d_wft_typ_subst : subtyping.
 Hint Resolve d_wft_typ_subst_stvar : subtyping.
 Hint Resolve d_wf_env_subst_tvar_typ : subtyping.
 
-Inductive d_sub_tvar_open_inv : typvar -> dtyp -> Prop :=
-| d__stoi__refl : forall X, d_sub_tvar_open_inv X (dtyp_var_f X)
+Inductive d_sub_tvar_open_inv : typvar -> typ -> Prop :=
+| d__stoi__refl : forall X, d_sub_tvar_open_inv X (typ_var_f X)
 | d__stoi__union : forall X T1 T2,
     d_sub_tvar_open_inv X T1 ->
     d_sub_tvar_open_inv X T2 ->
-    d_sub_tvar_open_inv X (dtyp_union T1 T2)
+    d_sub_tvar_open_inv X (typ_union T1 T2)
 | d__stoi__intersection1 : forall X T1 T2,
     d_sub_tvar_open_inv X T1 ->
-    d_sub_tvar_open_inv X (dtyp_intersection T1 T2)
+    d_sub_tvar_open_inv X (typ_intersection T1 T2)
 | d__stoi__intersection2 : forall X T1 T2,
     d_sub_tvar_open_inv X T2 ->
-    d_sub_tvar_open_inv X (dtyp_intersection T1 T2).
+    d_sub_tvar_open_inv X (typ_intersection T1 T2).
 
 Lemma d_sub_tvar_open_inv_subst : forall X1 X2 S1 T1,
   d_sub_tvar_open_inv X1 T1 ->
@@ -145,52 +145,51 @@ Proof.
 Qed.
 
 
-Inductive d_sub_tvar_inv : dtyp -> Prop :=
+Inductive d_sub_tvar_inv : typ -> Prop :=
 | d__sti__all : forall L T,
     (forall X, X `notin` L -> d_sub_tvar_open_inv X (T ^ᵈ X)) ->
-    d_sub_tvar_inv (dtyp_all T).
+    d_sub_tvar_inv (typ_all T).
 
 
 
-Fixpoint d_typ_order (T : dtyp) : nat :=
+Fixpoint d_typ_order (T : typ) : nat :=
   match T with
-  | dtyp_all T1 => S ( d_typ_order T1 )
-  | dtyp_arrow T1 T2 => d_typ_order T1 + d_typ_order T2
-  | dtyp_intersection T1 T2 => d_typ_order T1 + d_typ_order T2
-  | dtyp_union T1 T2 => d_typ_order T1 + d_typ_order T2
+  | typ_all T1 => S ( d_typ_order T1 )
+  | typ_arrow T1 T2 => d_typ_order T1 + d_typ_order T2
+  | typ_intersection T1 T2 => d_typ_order T1 + d_typ_order T2
+  | typ_union T1 T2 => d_typ_order T1 + d_typ_order T2
   | _ => 0
   end.
 
-Fixpoint d_typ_size (T : dtyp) :=
+Fixpoint d_typ_size (T : typ) :=
   match T with
-  | dtyp_intersection T1 T2 => 1 + d_typ_size T1 + d_typ_size T2
-  | dtyp_union T1 T2 => 1 + d_typ_size T1 + d_typ_size T2
+  | typ_intersection T1 T2 => 1 + d_typ_size T1 + d_typ_size T2
+  | typ_union T1 T2 => 1 + d_typ_size T1 + d_typ_size T2
   | _ => 0
   end.
 
 
-Lemma dmono_type_order_0 : forall T,
-  dmono_typ T -> d_typ_order T = 0.
+Lemma d_mono_type_order_0 : forall E T,
+  d_mono_typ E T -> d_typ_order T = 0.
 Proof.
   intros; induction H; simpl; auto.
-  - rewrite IHdmono_typ1. rewrite IHdmono_typ2. auto.
-  - rewrite IHdmono_typ1. rewrite IHdmono_typ2. auto.
-  - rewrite IHdmono_typ1. rewrite IHdmono_typ2. auto.
+  - rewrite IHd_mono_typ1. rewrite IHd_mono_typ2. auto.
+  - rewrite IHd_mono_typ1. rewrite IHd_mono_typ2. auto.
+  - rewrite IHd_mono_typ1. rewrite IHd_mono_typ2. auto.
 Qed.
 
-Lemma d_open_rec_mono_same_order : forall T1 T2 n,
-  dmono_typ T2 ->
-  d_typ_order (open_dtyp_wrt_dtyp_rec n T2 T1) = d_typ_order T1.
+Lemma d_open_rec_mono_same_order : forall E T1 T2 n,
+  d_mono_typ E T2 ->
+  d_typ_order (open_typ_wrt_typ_rec n T2 T1) = d_typ_order T1.
 Proof.
   induction T1; simpl; intros; auto.
   - destruct (lt_eq_lt_dec n n0).
-    + destruct s; auto. apply dmono_type_order_0; auto.
+    + destruct s; auto. eapply d_mono_type_order_0; eauto.
     + auto.
 Qed.
 
-
-Lemma d_open_rec_svar_same_order : forall T1 SX n,
-  d_typ_order (open_dtyp_wrt_dtyp_rec n (dtyp_svar SX) T1) = d_typ_order T1.
+Lemma d_open_rec_tvar_same_order : forall T1 X n,
+  d_typ_order (open_typ_wrt_typ_rec n (typ_var_f X) T1) = d_typ_order T1.
 Proof.
   induction T1; simpl; intros; auto.
   - destruct (lt_eq_lt_dec n n0).
@@ -198,27 +197,26 @@ Proof.
     + auto.
 Qed.
 
-
-Lemma d_open_mono_same_order : forall T1 T2,
-  dmono_typ T2 ->
-  d_typ_order (T1 ^^ᵈ T2) = d_typ_order T1.
+Lemma d_open_mono_same_order : forall E A1 T1,
+  d_mono_typ E T1 ->
+  d_typ_order (A1 ^^ᵈ T1) = d_typ_order A1.
 Proof.
-  intros. unfold open_dtyp_wrt_dtyp. apply d_open_rec_mono_same_order; auto.
+  intros. unfold open_typ_wrt_typ. eapply d_open_rec_mono_same_order; eauto.
 Qed.
 
 
-Lemma d_open_svar_same_order : forall T1 SX,
-  d_typ_order (T1 ^^ᵈ (dtyp_svar SX)) = d_typ_order T1.
+Lemma d_open_svar_same_order : forall T1 X,
+  d_typ_order (T1 ^ᵈ X) = d_typ_order T1.
 Proof.
-  intros. unfold open_dtyp_wrt_dtyp. apply d_open_rec_svar_same_order; auto.
+  intros. unfold open_typ_wrt_typ. apply d_open_rec_tvar_same_order; auto.
 Qed.
 
 
 Theorem d_sub_tvar_inv_nested_all_false: forall L1 L2 L3 T1 S1,
-  (forall X : atom, X `notin` L1 -> d_sub_tvar_open_inv X (open_dtyp_wrt_dtyp_rec 1 S1 T1 ^ᵈ X)) ->
-  (forall X : atom, X `notin` L2 -> ds_in X (dtyp_all (open_dtyp_wrt_dtyp_rec 1 `ᵈ X T1))) ->
-  (forall X : atom, X `notin` L3 -> ds_in X (open_dtyp_wrt_dtyp_rec 1 S1 T1 ^ᵈ X)) ->
-  lc_dtyp S1 ->
+  (forall X : atom, X `notin` L1 -> d_sub_tvar_open_inv X (open_typ_wrt_typ_rec 1 S1 T1 ^ᵈ X)) ->
+  (forall X : atom, X `notin` L2 -> ds_in X (typ_all (open_typ_wrt_typ_rec 1 `ᵈ X T1))) ->
+  (forall X : atom, X `notin` L3 -> ds_in X (open_typ_wrt_typ_rec 1 S1 T1 ^ᵈ X)) ->
+  lc_typ S1 ->
   False.
 Proof.
   intros. induction T1; simpl in *.
@@ -233,72 +231,71 @@ Proof.
         apply notin_union_2 in Fr0. apply notin_singleton_1 in Fr0. contradiction.
       * inst_cofinites_by L3.
         inversion H1.
-      * inst_cofinites_by (L3 `union` ftv_in_dtyp S1).
-        rewrite open_dtyp_wrt_dtyp_lc_dtyp in H1; auto.
+      * inst_cofinites_by (L3 `union` ftv_in_typ S1).
+        rewrite open_typ_wrt_typ_lc_typ in H1; auto.
         apply sin_in in H1. apply notin_union_2 in Fr. contradiction.
     + destruct (n - 1).
-      * unfold open_dtyp_wrt_dtyp in *. simpl in *.
+      * unfold open_typ_wrt_typ in *. simpl in *.
         inst_cofinites_by L2. dependent destruction H0.
         inst_cofinites_by (L `union` singleton X).
         dependent destruction H0.
         apply notin_union_2 in Fr0. apply notin_singleton_1 in Fr0. contradiction.
-      * unfold open_dtyp_wrt_dtyp in *. simpl in *.
+      * unfold open_typ_wrt_typ in *. simpl in *.
         inst_cofinites_by L3. inversion H1.
   - inst_cofinites_by (L3 `union` singleton X).
     dependent destruction H1. apply notin_union_2 in Fr. apply notin_singleton_1 in Fr. contradiction.
-  - inst_cofinites_by L3. inversion H1.
   - inst_cofinites_by L1. inversion H.
   - inst_cofinites_by L1. inversion H.
-  - assert (forall X : atom, X `notin` L1 -> d_sub_tvar_open_inv X (open_dtyp_wrt_dtyp_rec 1 S1 T1_1 ^ᵈ X)). {
+  - assert (forall X : atom, X `notin` L1 -> d_sub_tvar_open_inv X (open_typ_wrt_typ_rec 1 S1 T1_1 ^ᵈ X)). {
       intros. inst_cofinites_with X. inversion H; auto.
     }
-    assert (forall X : atom, X `notin` L2 -> ds_in X (dtyp_all (open_dtyp_wrt_dtyp_rec 1 `ᵈ X T1_1))).
+    assert (forall X : atom, X `notin` L2 -> ds_in X (typ_all (open_typ_wrt_typ_rec 1 `ᵈ X T1_1))).
     { intros. inst_cofinites_with X. dependent destruction H0.
       eapply dsin_all with (L:=L). intros. inst_cofinites_with Y.
       inversion H0. auto.
     }
-    assert  (forall X : atom, X `notin` L3 -> ds_in X (open_dtyp_wrt_dtyp_rec 1 S1 T1_1 ^ᵈ X)).
+    assert  (forall X : atom, X `notin` L3 -> ds_in X (open_typ_wrt_typ_rec 1 S1 T1_1 ^ᵈ X)).
     { intros. inst_cofinites_with X. inversion H1; auto.
     }
     auto.
-  - assert ((forall X : atom, X `notin` L1 -> d_sub_tvar_open_inv X (open_dtyp_wrt_dtyp_rec 1 S1 T1_1 ^ᵈ X)) \/
-            (forall X : atom, X `notin` L1 -> d_sub_tvar_open_inv X (open_dtyp_wrt_dtyp_rec 1 S1 T1_2 ^ᵈ X))).
+  - assert ((forall X : atom, X `notin` L1 -> d_sub_tvar_open_inv X (open_typ_wrt_typ_rec 1 S1 T1_1 ^ᵈ X)) \/
+            (forall X : atom, X `notin` L1 -> d_sub_tvar_open_inv X (open_typ_wrt_typ_rec 1 S1 T1_2 ^ᵈ X))).
     {
       intros.
-      inst_cofinites_by (L1 `union` ftv_in_dtyp (open_dtyp_wrt_dtyp_rec 1 S1 T1_1) `union`
-                                    ftv_in_dtyp (open_dtyp_wrt_dtyp_rec 1 S1 T1_2)).
+      inst_cofinites_by (L1 `union` ftv_in_typ (open_typ_wrt_typ_rec 1 S1 T1_1) `union`
+                                    ftv_in_typ (open_typ_wrt_typ_rec 1 S1 T1_2)).
       dependent destruction H.
       - left. intros. inst_cofinites_with X.
-        assert (d_sub_tvar_open_inv x (open_dtyp_wrt_dtyp_rec 1 S1 T1_1 ^ᵈ x)) by auto.
-        replace (open_dtyp_wrt_dtyp_rec 1 S1 T1_1 ^ᵈ X) with ({`ᵈ X /ᵈ x}(open_dtyp_wrt_dtyp_rec 1 S1 T1_1 ^ᵈ x)).
+        assert (d_sub_tvar_open_inv x (open_typ_wrt_typ_rec 1 S1 T1_1 ^ᵈ x)) by auto.
+        replace (open_typ_wrt_typ_rec 1 S1 T1_1 ^ᵈ X) with ({`ᵈ X /ᵈ x}(open_typ_wrt_typ_rec 1 S1 T1_1 ^ᵈ x)).
         now apply d_sub_tvar_open_inv_subst_var.
-        rewrite d_subst_tv_in_dtyp_open_dtyp_wrt_dtyp; auto.
-        rewrite (d_subst_tv_in_dtyp_fresh_eq); auto. simpl.
+        rewrite subst_tvar_in_typ_open_typ_wrt_typ; auto.
+        rewrite (subst_tvar_in_typ_fresh_eq); auto. simpl.
         unfold eq_dec. destruct (EqDec_eq_of_X x x); auto. contradiction.
       - right. intros. inst_cofinites_with X.
-        assert (d_sub_tvar_open_inv x (open_dtyp_wrt_dtyp_rec 1 S1 T1_2 ^ᵈ x)) by auto.
-        replace (open_dtyp_wrt_dtyp_rec 1 S1 T1_2 ^ᵈ X) with ({`ᵈ X /ᵈ x}(open_dtyp_wrt_dtyp_rec 1 S1 T1_2 ^ᵈ x)).
+        assert (d_sub_tvar_open_inv x (open_typ_wrt_typ_rec 1 S1 T1_2 ^ᵈ x)) by auto.
+        replace (open_typ_wrt_typ_rec 1 S1 T1_2 ^ᵈ X) with ({`ᵈ X /ᵈ x}(open_typ_wrt_typ_rec 1 S1 T1_2 ^ᵈ x)).
         now apply d_sub_tvar_open_inv_subst_var.
-        rewrite d_subst_tv_in_dtyp_open_dtyp_wrt_dtyp; auto.
-        rewrite (d_subst_tv_in_dtyp_fresh_eq); auto. simpl.
+        rewrite subst_tvar_in_typ_open_typ_wrt_typ; auto.
+        rewrite (subst_tvar_in_typ_fresh_eq); auto. simpl.
         unfold eq_dec. destruct (EqDec_eq_of_X x x); auto. contradiction.
     }
     inversion H3.
-    + assert (forall X : atom, X `notin` L2 -> ds_in X (dtyp_all (open_dtyp_wrt_dtyp_rec 1 `ᵈ X T1_1))).
+    + assert (forall X : atom, X `notin` L2 -> ds_in X (typ_all (open_typ_wrt_typ_rec 1 `ᵈ X T1_1))).
       { intros. inst_cofinites_with X. dependent destruction H0.
         eapply dsin_all with (L:=L). intros. inst_cofinites_with Y.
         inversion H0. auto.
       }
-      assert  (forall X, X `notin` L3 -> ds_in X (open_dtyp_wrt_dtyp_rec 1 S1 T1_1 ^ᵈ X)).
+      assert  (forall X, X `notin` L3 -> ds_in X (open_typ_wrt_typ_rec 1 S1 T1_1 ^ᵈ X)).
       { intros. inst_cofinites_with X. inversion H1; auto.
       }
       auto.
-    + assert (forall X, X `notin` L2 -> ds_in X (dtyp_all (open_dtyp_wrt_dtyp_rec 1 `ᵈ X T1_2))).
+    + assert (forall X, X `notin` L2 -> ds_in X (typ_all (open_typ_wrt_typ_rec 1 `ᵈ X T1_2))).
       { intros. inst_cofinites_with X. dependent destruction H0.
         eapply dsin_all with (L:=L). intros. inst_cofinites_with Y.
         inversion H0. auto.
       }
-      assert  (forall X, X `notin` L3 -> ds_in X (open_dtyp_wrt_dtyp_rec 1 S1 T1_2 ^ᵈ X)).
+      assert  (forall X, X `notin` L3 -> ds_in X (open_typ_wrt_typ_rec 1 S1 T1_2 ^ᵈ X)).
       { intros. inst_cofinites_with X. inversion H1; auto.
       }
       auto.
@@ -311,7 +308,7 @@ Theorem d_sub_tvar_ind_open_inv_complete: forall n1 n2 E S1 T1 X L,
     E ⊢ T1 ^^ᵈ S1 <: `ᵈ X ->
     (forall X, X `notin` L -> ds_in X (T1 ^ᵈ X)) ->
     dmono_typ S1 ->
-    d_sub_tvar_inv (dtyp_all T1).
+    d_sub_tvar_inv (typ_all T1).
 Proof.
     intro n1. induction n1.
     - intros. inversion H.
@@ -321,19 +318,19 @@ Proof.
         * rename H3 into Hdsin. rename H4 into Hmono. destruct T1; simpl in *; try solve [inversion Heq].
           -- inst_cofinites_by L. inversion Hdsin.
           -- destruct n. simpl in *.
-             ++ unfold open_dtyp_wrt_dtyp in Heq. simpl in Heq. subst. inversion Hmono.
-             ++ unfold open_dtyp_wrt_dtyp in Heq. simpl in Heq. inversion Heq.
+             ++ unfold open_typ_wrt_typ in Heq. simpl in Heq. subst. inversion Hmono.
+             ++ unfold open_typ_wrt_typ in Heq. simpl in Heq. inversion Heq.
         * rename H3 into Hdsin. rename H4 into Hmono. destruct T1; simpl in *; try solve [inversion Heq].
           -- destruct n. simpl in *.
              ++ eapply d__sti__all with (L:=L). intros. constructor.
-             ++ unfold open_dtyp_wrt_dtyp in Heq. simpl in Heq. inversion Heq.
+             ++ unfold open_typ_wrt_typ in Heq. simpl in Heq. inversion Heq.
           -- inst_cofinites_by (L `union` (singleton X0)).
-            unfold open_dtyp_wrt_dtyp in Hdsin. simpl in Hdsin. dependent destruction Hdsin.
+            unfold open_typ_wrt_typ in Hdsin. simpl in Hdsin. dependent destruction Hdsin.
             apply notin_union_2 in Fr. apply notin_singleton_1 in Fr. contradiction.
         * rename H3 into Hdsin. rename H4 into Hmono. destruct T1; simpl in *; try solve [inversion Heq].
           -- destruct n. simpl in *.
              ++ eapply d__sti__all with (L:=L). intros. constructor.
-             ++ unfold open_dtyp_wrt_dtyp in Heq. simpl in Heq. inversion Heq.
+             ++ unfold open_typ_wrt_typ in Heq. simpl in Heq. inversion Heq.
           -- exfalso.
              dependent destruction Heq.
              eapply IHn1 in H7; eauto. inversion H7. auto.
@@ -342,56 +339,56 @@ Proof.
         * rename H3 into Hdsin. rename H4 into Hmono. destruct T1; simpl in *; try solve [inversion Heq].
           -- destruct n. simpl in *.
              ++ eapply d__sti__all with (L:=L). intros. constructor.
-             ++ unfold open_dtyp_wrt_dtyp in Heq. simpl in Heq. inversion Heq.
+             ++ unfold open_typ_wrt_typ in Heq. simpl in Heq. inversion Heq.
           -- dependent destruction Heq. apply IHn2 with (L:=L) in H1.
              dependent destruction H1.
              eapply d__sti__all with (L:=L `union` L0); auto.
              intros. inst_cofinites_with X0. eapply d__stoi__intersection1; eauto.
-             ++ unfold open_dtyp_wrt_dtyp. lia.
-             ++ unfold open_dtyp_wrt_dtyp. lia.
+             ++ unfold open_typ_wrt_typ. lia.
+             ++ unfold open_typ_wrt_typ. lia.
              ++ intros. inst_cofinites_with X0.  dependent destruction Hdsin. auto.
              ++ auto.
         * rename H3 into Hdsin. rename H4 into Hmono. destruct T1; simpl in *; try solve [inversion Heq].
           -- destruct n. simpl in *.
              ++ eapply d__sti__all with (L:=L). intros. constructor.
-             ++ unfold open_dtyp_wrt_dtyp in Heq. simpl in Heq. inversion Heq.
+             ++ unfold open_typ_wrt_typ in Heq. simpl in Heq. inversion Heq.
           -- dependent destruction Heq. apply IHn2 with (L:=L) in H1.
              dependent destruction H1.
              eapply d__sti__all with (L:=L `union` L0); auto.
              intros. inst_cofinites_with X0. eapply d__stoi__intersection2; eauto.
-             ++ unfold open_dtyp_wrt_dtyp. lia.
-             ++ unfold open_dtyp_wrt_dtyp. lia.
+             ++ unfold open_typ_wrt_typ. lia.
+             ++ unfold open_typ_wrt_typ. lia.
              ++ intros. inst_cofinites_with X0.  dependent destruction Hdsin. auto.
              ++ auto.
         * rename H2 into Hdsin. rename H3 into Hmono. destruct T1; simpl in *; try solve [inversion Heq].
           -- destruct n. simpl in *.
              ++ eapply d__sti__all with (L:=L). intros. constructor.
-             ++ unfold open_dtyp_wrt_dtyp in Heq. simpl in Heq. inversion Heq.
+             ++ unfold open_typ_wrt_typ in Heq. simpl in Heq. inversion Heq.
           -- dependent destruction Heq.
              eapply IHn2 with (L:=L) in H1_; eauto...
              eapply IHn2 with (L:=L) in H1_0; eauto...
              ++ dependent destruction H1_.
                 dependent destruction H1_0.
                 eapply d__sti__all with (L:=L `union` L0 `union` L1). intros.
-                replace (dtyp_union T1_1 T1_2 ^ᵈ X0) with (dtyp_union (T1_1 ^ᵈ X0) (T1_2 ^ᵈ X0)) by auto.
+                replace (typ_union T1_1 T1_2 ^ᵈ X0) with (typ_union (T1_1 ^ᵈ X0) (T1_2 ^ᵈ X0)) by auto.
                 econstructor; eauto.
-              ++ unfold open_dtyp_wrt_dtyp. lia.
-              ++ unfold open_dtyp_wrt_dtyp. lia.
+              ++ unfold open_typ_wrt_typ. lia.
+              ++ unfold open_typ_wrt_typ. lia.
               ++ intros. inst_cofinites_with X0. dependent destruction Hdsin; auto.
-              ++ unfold open_dtyp_wrt_dtyp. lia.
-              ++ unfold open_dtyp_wrt_dtyp. lia.
+              ++ unfold open_typ_wrt_typ. lia.
+              ++ unfold open_typ_wrt_typ. lia.
               ++ intros. inst_cofinites_with X0. dependent destruction Hdsin; auto.
 Qed.
 
 
 Lemma d_sub_tvar_inv_subst: forall T1 X S1,
-    d_sub_tvar_inv T1 -> lc_dtyp S1 -> d_sub_tvar_inv ({S1 /ᵈ X} T1).
+    d_sub_tvar_inv T1 -> lc_typ S1 -> d_sub_tvar_inv ({S1 /ᵈ X} T1).
 Proof.
   intros. dependent destruction H.
   simpl.
   eapply d__sti__all with (L:=L `union` singleton X).
   intros.
-  rewrite dtyp_subst_open_comm.
+  rewrite typ_subst_open_comm.
   - apply d_sub_tvar_open_inv_subst; auto.
   - auto.
   - simpl. apply notin_union_2 in H1.
@@ -400,13 +397,13 @@ Proof.
 Qed.
 
 
-Inductive d_ord_mono : dtyp -> Prop :=
-| d__ordmono__tvar : forall X, d_ord_mono (dtyp_var_f X)
-| d__ordmono__unit : d_ord_mono dtyp_unit
+Inductive d_ord_mono : typ -> Prop :=
+| d__ordmono__tvar : forall X, d_ord_mono (typ_var_f X)
+| d__ordmono__unit : d_ord_mono typ_unit
 | d__ordmono__arr : forall T1 T2,
     dmono_typ T1 ->
     dmono_typ T2 ->
-    d_ord_mono (dtyp_arrow T1 T2)
+    d_ord_mono (typ_arrow T1 T2)
 .
 
 Lemma d_ord_mono_neq_intersection: forall T1,
@@ -423,18 +420,18 @@ Proof.
   intros. induction H; auto.
 Qed.
 
-Inductive d_mono_ordiu : dtyp -> Prop :=
+Inductive d_mono_ordiu : typ -> Prop :=
 | d__monoord__base : forall T1,
     d_ord_mono T1 ->
     d_mono_ordiu T1
 | d__monoord__union : forall T1 T2,
     d_mono_ordiu T1 ->
     d_mono_ordiu T2 ->
-    d_mono_ordiu (dtyp_union T1 T2)
+    d_mono_ordiu (typ_union T1 T2)
 | d__monoord__inter : forall T1 T2,
     d_mono_ordiu T1 ->
     d_mono_ordiu T2 ->
-    d_mono_ordiu (dtyp_intersection T1 T2).
+    d_mono_ordiu (typ_intersection T1 T2).
 
 
 Lemma d_mono_ordiu_complete : forall T1,
@@ -550,11 +547,11 @@ Admitted. *)
 
 Theorem d_sub_tvar_ind_sub_all : forall E T1 T2,
   ⊢ E ->
-  d_sub_tvar_inv (dtyp_all T1) ->
-  E ⊢ dtyp_all T1 ->
-  dmono_typ T2 ->
+  d_sub_tvar_inv (typ_all T1) ->
+  E ⊢ typ_all T1 ->
+  d_mono_typ E T2 ->
   E ⊢ T2 ->
-  E ⊢ dtyp_all T1 <: T2.
+  E ⊢ typ_all T1 <: T2.
 Proof.
   intros * Hwfenv H Hwft Hmono Hwft2.
   specialize (d_mono_ordiu_complete _ Hmono). intros.
@@ -568,10 +565,10 @@ Proof.
     + auto.
     + auto.
     + auto.
-    + inst_cofinites_by (L `union` L0 `union` ftv_in_dtyp T1 `union` dom E) using_name X.
+    + inst_cofinites_by (L `union` L0 `union` ftv_in_typ T1 `union` dom E) using_name X.
       apply d_sub_tvar_ind_open_subst with (E:= E) (T2:=T0) (F:=nil) in H.
-      rewrite d_subst_tv_in_dtyp_open_dtyp_wrt_dtyp in H; auto.
-      rewrite d_subst_tv_in_dtyp_fresh_eq in H; auto.
+      rewrite d_subst_tv_in_typ_open_typ_wrt_typ in H; auto.
+      rewrite d_subst_tv_in_typ_fresh_eq in H; auto.
       simpl in H. destruct eq_dec in H. auto.
       contradiction.
       * simpl. constructor; auto.
@@ -595,45 +592,45 @@ Proof with eauto with subtyping.
   - eapply dsub_refl; auto...
   - eapply dsub_refl; auto...
   - simpl. eapply d_sub_all with (L:=L `union` singleton X `union` dom E `union` dom F); intros SX Hfr; inst_cofinites_with SX.
-    + rewrite dtyp_subst_open_comm; auto...
-      apply fstv_sin_dtyp_subst_tv; auto...
-    + rewrite dtyp_subst_open_comm; auto...
-      apply fstv_sin_dtyp_subst_tv; auto...
-    + inst_cofinites_with SX. repeat rewrite dtyp_subst_open_comm; eauto...
+    + rewrite typ_subst_open_comm; auto...
+      apply fstv_sin_typ_subst_tv; auto...
+    + rewrite typ_subst_open_comm; auto...
+      apply fstv_sin_typ_subst_tv; auto...
+    + inst_cofinites_with SX. repeat rewrite typ_subst_open_comm; eauto...
       replace (SX ~ dbind_stvar_empty ++ map (d_subst_tv_in_binding T2 X) F ++ E) with
       (map (d_subst_tv_in_binding T2 X) (SX ~ dbind_stvar_empty ++ F) ++ E) by auto.
       eapply H2; auto... simpl. constructor; eauto.
   - destruct T1 eqn:HeqT.
     + eapply d_sub_alll with (L:=L `union` singleton X) (T2:={T2 /ᵈ X} T0); auto...
-      * intros. inst_cofinites_with X0. rewrite dtyp_subst_open_comm; auto...
-        apply ftv_sin_dtyp_subst_inv; auto...
+      * intros. inst_cofinites_with X0. rewrite typ_subst_open_comm; auto...
+        apply ftv_sin_typ_subst_inv; auto...
       * apply d_mono_typ_subst_mono_mono; auto.
-      * rewrite <- d_subst_tv_in_dtyp_open_dtyp_wrt_dtyp; eauto...
+      * rewrite <- d_subst_tv_in_typ_open_typ_wrt_typ; eauto...
     + eapply d_sub_alll with (L:=L `union` singleton X) (T2:={T2 /ᵈ X} T0); eauto...
-      * intros. inst_cofinites_with X0. rewrite dtyp_subst_open_comm; auto...
-        apply ftv_sin_dtyp_subst_inv; auto...
+      * intros. inst_cofinites_with X0. rewrite typ_subst_open_comm; auto...
+        apply ftv_sin_typ_subst_inv; auto...
       * apply d_mono_typ_subst_mono_mono; auto.
-      * rewrite <- d_subst_tv_in_dtyp_open_dtyp_wrt_dtyp; eauto...
+      * rewrite <- d_subst_tv_in_typ_open_typ_wrt_typ; eauto...
     + eapply d_sub_alll with (L:=L `union` singleton X) (T2:={T2 /ᵈ X} T0); auto...
-      * intros. inst_cofinites_with X0. rewrite dtyp_subst_open_comm; auto...
-        apply ftv_sin_dtyp_subst_inv; auto...
+      * intros. inst_cofinites_with X0. rewrite typ_subst_open_comm; auto...
+        apply ftv_sin_typ_subst_inv; auto...
       * apply d_mono_typ_subst_mono_mono; auto.
-      * rewrite <- d_subst_tv_in_dtyp_open_dtyp_wrt_dtyp; eauto...
+      * rewrite <- d_subst_tv_in_typ_open_typ_wrt_typ; eauto...
     + apply d_sub_dwft in Hsub as Hwft1. destruct Hwft1 as [_ [HwftS HwftT]]. inversion HwftT.
     + simpl.
       apply d_sub_dwft in Hsub as Hwft1. destruct Hwft1 as [_ [HwftS HwftT]].
       apply d_sub_tvar_ind_sub_all.
       -- eapply d_wf_env_subst_tvar_typ; auto.
-      -- replace (dtyp_all ({T2 /ᵈ X} S1)) with ({T2 /ᵈ X} (dtyp_all S1)) by auto.
+      -- replace (typ_all ({T2 /ᵈ X} S1)) with ({T2 /ᵈ X} (typ_all S1)) by auto.
          apply d_sub_tvar_inv_subst. eapply d_sub_tvar_ind_open_inv_complete; eauto.
-         eapply dwf_typ_lc_dtyp; eauto.
-      -- replace (dtyp_all ({T2 /ᵈ X} S1)) with ({T2 /ᵈ X} (dtyp_all S1)) by auto.
+         eapply dwf_typ_lc_typ; eauto.
+      -- replace (typ_all ({T2 /ᵈ X} S1)) with ({T2 /ᵈ X} (typ_all S1)) by auto.
          apply d_wft_typ_subst; auto.
          inst_cofinites_for dwftyp_all.
          ++ auto.
          ++ intros. eapply dwf_typ_open_inv with (X:=X1) (S1:=T0); auto.
-            rewrite d_subst_tv_in_dtyp_open_dtyp_wrt_dtyp; auto.
-            simpl. rewrite (d_subst_tv_in_dtyp_fresh_eq); auto.
+            rewrite d_subst_tv_in_typ_open_typ_wrt_typ; auto.
+            simpl. rewrite (d_subst_tv_in_typ_fresh_eq); auto.
             unfold eq_dec. destruct (EqDec_eq_of_X X1 X1); auto.
             ** apply dwf_typ_weakening_cons; auto.
             ** contradiction.
@@ -642,21 +639,21 @@ Proof with eauto with subtyping.
          apply d_wft_typ_subst; auto.
     + apply d_sub_dwft in Hsub as Hwft1. destruct Hwft1 as [_ [HwftS HwftT]]. inversion HwftT.
       eapply d_sub_alll with (L:=L `union` singleton X) (T2:={T2 /ᵈ X} T0); eauto...
-      * intros. inst_cofinites_with X0. rewrite dtyp_subst_open_comm; auto...
-        apply ftv_sin_dtyp_subst_inv; auto...
+      * intros. inst_cofinites_with X0. rewrite typ_subst_open_comm; auto...
+        apply ftv_sin_typ_subst_inv; auto...
       * apply d_mono_typ_subst_mono_mono; auto.
-      * rewrite <- d_subst_tv_in_dtyp_open_dtyp_wrt_dtyp; eauto...
+      * rewrite <- d_subst_tv_in_typ_open_typ_wrt_typ; eauto...
     + eapply d_sub_alll with (L:=L `union` singleton X) (T2:={T2 /ᵈ X} T0); eauto...
       * simpl. dependent destruction H.
-        constructor; apply d_subst_tv_in_dtyp_lc_dtyp; auto.
+        constructor; apply d_subst_tv_in_typ_lc_typ; auto.
       * simpl. dependent destruction H0.
-        constructor; apply d_subst_tv_in_dtyp_lc_dtyp; auto.
+        constructor; apply d_subst_tv_in_typ_lc_typ; auto.
       * simpl. dependent destruction H0.
-        constructor; apply d_subst_tv_in_dtyp_lc_dtyp; auto.
-      * intros. inst_cofinites_with X0. rewrite dtyp_subst_open_comm; auto...
-        apply ftv_sin_dtyp_subst_inv; auto...
+        constructor; apply d_subst_tv_in_typ_lc_typ; auto.
+      * intros. inst_cofinites_with X0. rewrite typ_subst_open_comm; auto...
+        apply ftv_sin_typ_subst_inv; auto...
       * apply d_mono_typ_subst_mono_mono; auto.
-      * rewrite <- d_subst_tv_in_dtyp_open_dtyp_wrt_dtyp; eauto...
+      * rewrite <- d_subst_tv_in_typ_open_typ_wrt_typ; eauto...
     + inversion H.
     + inversion H1.
     + inversion H0.
@@ -665,14 +662,14 @@ Qed.
 
 Hint Resolve d_wft_typ_subst_stvar : subtyping.
 Hint Resolve d_wf_env_subst_stvar_typ : subtyping.
-Hint Resolve dsubst_stv_lc_dtyp : lngen.
+Hint Resolve dsubst_stv_lc_typ : lngen.
 
 Lemma dneq_all_intersection_union_subst_stv : forall T1 T2 SX,
-  lc_dtyp T1 -> lc_dtyp T2 ->
+  lc_typ T1 -> lc_typ T2 ->
   dneq_all T1 -> dneq_intersection T1 -> dneq_union T1 ->
   (dneq_all ({T2 /ₛᵈ SX} T1) /\
    dneq_intersection ({T2 /ₛᵈ SX} T1) /\
-   dneq_union ({T2 /ₛᵈ SX} T1)) \/ T1 = dtyp_svar SX.
+   dneq_union ({T2 /ₛᵈ SX} T1)) \/ T1 = typ_svar SX.
 Proof with eauto with lngen.
   intros. destruct T1; simpl in *; auto...
   - destruct (SX0 == SX); subst; auto.
@@ -686,7 +683,7 @@ Qed.
 
 Theorem d_sub_mono_stvar_false : forall E T1 SX,
   dmono_typ T1 ->
-  E ⊢ T1 <: dtyp_svar SX ->
+  E ⊢ T1 <: typ_svar SX ->
   False.
 Proof.
   intros. induction H; try solve [(dependent destruction H0); auto].
@@ -696,7 +693,7 @@ Qed.
 Theorem d_sub_open_mono_stvar_false: forall n1 n2 E S1 T1 SX L,
     d_typ_order (T1 ^^ᵈ S1) < n1 ->
     d_typ_size (T1 ^^ᵈ S1) < n2 ->
-    E ⊢ T1 ^^ᵈ S1 <: dtyp_svar SX ->
+    E ⊢ T1 ^^ᵈ S1 <: typ_svar SX ->
     (forall X, X `notin` L -> ds_in X (T1 ^ᵈ X)) ->
     dmono_typ S1 ->
     False.
@@ -709,60 +706,60 @@ Proof.
       * destruct T1; simpl in *; try solve [inversion Heq].
         -- inst_cofinites_by L using_name X. inversion H3.
         -- destruct n.
-           ++ unfold open_dtyp_wrt_dtyp in Heq. simpl in *.
+           ++ unfold open_typ_wrt_typ in Heq. simpl in *.
               subst. inversion H4.
-           ++ unfold open_dtyp_wrt_dtyp in Heq. simpl in *.
+           ++ unfold open_typ_wrt_typ in Heq. simpl in *.
               inversion Heq.
       * destruct T1; simpl in *; try solve [inversion Heq].
         -- destruct n.
-          ++ unfold open_dtyp_wrt_dtyp in Heq. simpl in *.
+          ++ unfold open_typ_wrt_typ in Heq. simpl in *.
             subst. inversion H4.
-          ++ unfold open_dtyp_wrt_dtyp in Heq. simpl in *.
+          ++ unfold open_typ_wrt_typ in Heq. simpl in *.
             inversion Heq.
         -- inst_cofinites_by L using_name X. inversion H3.
       * destruct T1; simpl in *; try solve [inversion Heq].
         -- destruct n.
-          ++ unfold open_dtyp_wrt_dtyp in Heq. simpl in Heq.
+          ++ unfold open_typ_wrt_typ in Heq. simpl in Heq.
               subst. dependent destruction H9.
-          ++ unfold open_dtyp_wrt_dtyp in Heq. simpl in Heq.
+          ++ unfold open_typ_wrt_typ in Heq. simpl in Heq.
              inversion Heq.
         -- dependent destruction Heq.
            eapply IHn1; eauto. rewrite d_open_mono_same_order; auto. lia.
       * destruct T1; simpl in *; try solve [inversion Heq].
         -- destruct n.
-           ++ unfold open_dtyp_wrt_dtyp in H, H0, Heq. simpl in *.
+           ++ unfold open_typ_wrt_typ in H, H0, Heq. simpl in *.
               subst. dependent destruction H4.
               apply d_sub_mono_stvar_false in H1; auto.
-           ++ unfold open_dtyp_wrt_dtyp in Heq. simpl in Heq.
+           ++ unfold open_typ_wrt_typ in Heq. simpl in Heq.
               inversion Heq.
-        -- dependent destruction Heq. unfold open_dtyp_wrt_dtyp in *.
+        -- dependent destruction Heq. unfold open_typ_wrt_typ in *.
            eapply IHn2 with (L:=L); eauto. lia. lia.
            intros. inst_cofinites_with X. dependent destruction H3; auto.
       * destruct T1; simpl in *; try solve [inversion Heq].
         -- destruct n.
-           ++ unfold open_dtyp_wrt_dtyp in H, H0, Heq. simpl in *.
+           ++ unfold open_typ_wrt_typ in H, H0, Heq. simpl in *.
               subst. dependent destruction H4.
               apply d_sub_mono_stvar_false in H1; auto.
-           ++ unfold open_dtyp_wrt_dtyp in Heq. simpl in Heq.
+           ++ unfold open_typ_wrt_typ in Heq. simpl in Heq.
              inversion Heq.
-        -- dependent destruction Heq. unfold open_dtyp_wrt_dtyp in *.
+        -- dependent destruction Heq. unfold open_typ_wrt_typ in *.
            eapply IHn2 with (L:=L); eauto. lia. lia.
            intros. inst_cofinites_with X. dependent destruction H3; auto.
       * destruct T1; simpl in *; try solve [inversion Heq].
         -- destruct n.
-           ++ unfold open_dtyp_wrt_dtyp in H, H0, Heq. simpl in *.
+           ++ unfold open_typ_wrt_typ in H, H0, Heq. simpl in *.
               subst. dependent destruction H3.
               apply d_sub_mono_stvar_false in H1_; auto.
-           ++ unfold open_dtyp_wrt_dtyp in Heq. simpl in Heq.
+           ++ unfold open_typ_wrt_typ in Heq. simpl in Heq.
              inversion Heq.
-        -- dependent destruction Heq. unfold open_dtyp_wrt_dtyp in *.
+        -- dependent destruction Heq. unfold open_typ_wrt_typ in *.
            eapply IHn2 with (L:=L); eauto. lia. lia.
            intros. inst_cofinites_with X. dependent destruction H2; auto.
 Qed.
 
 Theorem d_mono_notin_stvar : forall F E T SX,
   F ++ (SX ~ dbind_stvar_empty) ++ E ⊢ T -> dmono_typ T ->
-  SX `notin` fstv_in_dtyp T.
+  SX `notin` fstv_in_typ T.
 Proof.
   intros. induction H0; simpl in *; auto;
   dependent destruction H; auto.
@@ -777,23 +774,23 @@ Proof with subst; eauto using dwf_typ_weaken_head with subtyping.
   - eapply dsub_refl; auto...
   - eapply dsub_refl; auto...
   - simpl. inst_cofinites_for d_sub_all; intros SX1 Hfr; inst_cofinites_with SX1.
-    + rewrite d_subst_stv_in_dtyp_open_comm; auto...
-      apply fstv_sins_dtyp_subst_stv_s; auto...
-    + rewrite d_subst_stv_in_dtyp_open_comm; auto...
-      apply fstv_sins_dtyp_subst_stv_s; auto...
-    + repeat rewrite d_subst_stv_in_dtyp_open_comm; eauto...
+    + rewrite d_subst_stv_in_typ_open_comm; auto...
+      apply fstv_sins_typ_subst_stv_s; auto...
+    + rewrite d_subst_stv_in_typ_open_comm; auto...
+      apply fstv_sins_typ_subst_stv_s; auto...
+    + repeat rewrite d_subst_stv_in_typ_open_comm; eauto...
       replace (SX1 ~ dbind_stvar_empty ++ map (d_subst_stv_in_binding T2 SX) F ++ E) with
       (map (d_subst_stv_in_binding T2 SX) (SX1 ~ dbind_stvar_empty ++ F) ++ E) by auto.
       eapply H2; auto...
   - simpl. destruct (dneq_all_intersection_union_subst_stv T1 T2 SX) as [[? [? ?]] | ?]; eauto...
     + eapply d_sub_alll with (L:=L `union` singleton SX) (T2:={T2 /ₛᵈ SX} T0); eauto...
-      * intros. inst_cofinites_with SX0. rewrite d_subst_stv_in_dtyp_open_comm; auto...
-        apply fstv_sins_dtyp_subst_stv; auto...
+      * intros. inst_cofinites_with SX0. rewrite d_subst_stv_in_typ_open_comm; auto...
+        apply fstv_sins_typ_subst_stv; auto...
       * apply d_wft_typ_subst_stvar; auto...
         destruct (d_sub_dwft _ _ _ H5) as [? [? ?]]. auto.
-      * rewrite d_subst_stv_in_dtyp_fresh_eq; auto.
+      * rewrite d_subst_stv_in_typ_fresh_eq; auto.
         eapply d_mono_notin_stvar with (F := F) (E := E); auto.
-      * rewrite <- d_subst_stv_in_dtyp_open_dtyp_wrt_dtyp; eauto...
+      * rewrite <- d_subst_stv_in_typ_open_typ_wrt_typ; eauto...
     + eapply d_sub_open_mono_stvar_false in H5; eauto. contradiction.
   - simpl. apply d_sub_intersection2. eauto with subtyping.
     apply d_wft_typ_subst_stvar; auto...
@@ -809,68 +806,68 @@ Proof with subst; eauto using dwf_typ_weaken_head with subtyping.
     destruct (d_sub_dwft _ _ _ H) as [? [? ?]]. auto.
 Qed.
 
-Inductive d_sub_sized : denv -> dtyp -> dtyp -> nat -> Prop :=
- | d__subs__top : forall (E:denv) (S1:dtyp) (n:nat),
+Inductive d_sub_sized : denv -> typ -> typ -> nat -> Prop :=
+ | d__subs__top : forall (E:denv) (S1:typ) (n:nat),
      dwf_env E ->
      dwf_typ E S1 ->
-     d_sub_sized E S1 dtyp_top n
- | d__subs__bot : forall (E:denv) (T:dtyp) (n:nat),
+     d_sub_sized E S1 typ_top n
+ | d__subs__bot : forall (E:denv) (T:typ) (n:nat),
      dwf_env E ->
      dwf_typ E T ->
-     d_sub_sized E dtyp_bot T n
+     d_sub_sized E typ_bot T n
  | d__subs__unit : forall (E:denv) (n:nat),
      dwf_env E ->
-     d_sub_sized E dtyp_unit dtyp_unit n
+     d_sub_sized E typ_unit typ_unit n
  | d__subs__tvar : forall (E:denv) (X:typvar) (n:nat),
      dwf_env E ->
-     dwf_typ E (dtyp_var_f X) ->
-     d_sub_sized E (dtyp_var_f X) (dtyp_var_f X) n
+     dwf_typ E (typ_var_f X) ->
+     d_sub_sized E (typ_var_f X) (typ_var_f X) n
  | d__subs__stvar : forall (E:denv) (SX:stypvar) (n:nat),
      dwf_env E ->
-     dwf_typ E (dtyp_svar SX) ->
-     d_sub_sized E (dtyp_svar SX) (dtyp_svar SX) n
- | d__subs__arrow : forall (E:denv) (S1 S2 T1 T2:dtyp) (n1 n2:nat),
+     dwf_typ E (typ_svar SX) ->
+     d_sub_sized E (typ_svar SX) (typ_svar SX) n
+ | d__subs__arrow : forall (E:denv) (S1 S2 T1 T2:typ) (n1 n2:nat),
      d_sub_sized E T1 S1 n1 ->
      d_sub_sized E S2 T2 n2 ->
-     d_sub_sized E (dtyp_arrow S1 S2) (dtyp_arrow T1 T2) (S (n1 + n2))
- | d__subs__all : forall (L:vars) (E:denv) (S1 T1:dtyp) (n:nat),
-     ( forall SX , SX \notin L -> ds_in_s SX  (open_dtyp_wrt_dtyp  S1   (dtyp_svar SX) ) ) ->
-     ( forall SX , SX \notin L -> ds_in_s SX  (open_dtyp_wrt_dtyp  T1   (dtyp_svar SX) ) ) ->
-     ( forall SX , SX \notin L -> d_sub_sized  ( SX ~ dbind_stvar_empty  ++  E )   (open_dtyp_wrt_dtyp  S1   (dtyp_svar SX) )   (open_dtyp_wrt_dtyp  T1  (dtyp_svar SX) ) n) ->
-     d_sub_sized E (dtyp_all S1) (dtyp_all T1) (S n)
- | d__subs__alll : forall (L:vars) (E:denv) (S1 T1 T2:dtyp) (n:nat),
+     d_sub_sized E (typ_arrow S1 S2) (typ_arrow T1 T2) (S (n1 + n2))
+ | d__subs__all : forall (L:vars) (E:denv) (S1 T1:typ) (n:nat),
+     ( forall SX , SX \notin L -> ds_in_s SX  (open_typ_wrt_typ  S1   (typ_svar SX) ) ) ->
+     ( forall SX , SX \notin L -> ds_in_s SX  (open_typ_wrt_typ  T1   (typ_svar SX) ) ) ->
+     ( forall SX , SX \notin L -> d_sub_sized  ( SX ~ dbind_stvar_empty  ++  E )   (open_typ_wrt_typ  S1   (typ_svar SX) )   (open_typ_wrt_typ  T1  (typ_svar SX) ) n) ->
+     d_sub_sized E (typ_all S1) (typ_all T1) (S n)
+ | d__subs__alll : forall (L:vars) (E:denv) (S1 T1 T2:typ) (n:nat),
      dneq_all T1 ->
      dneq_intersection T1 ->
      dneq_union T1 ->
-     ( forall X , X \notin L -> ds_in X  (open_dtyp_wrt_dtyp  S1   (dtyp_var_f X) ) ) ->
+     ( forall X , X \notin L -> ds_in X  (open_typ_wrt_typ  S1   (typ_var_f X) ) ) ->
      dwf_typ E T2 ->
      dmono_typ T2 ->
-     d_sub_sized E  (open_dtyp_wrt_dtyp  S1   T2 )  T1 n ->
-     d_sub_sized E (dtyp_all S1) T1 (S n)
- | d__subs__intersection1 : forall (E:denv) (S1 T1 T2:dtyp) (n1 n2:nat),
+     d_sub_sized E  (open_typ_wrt_typ  S1   T2 )  T1 n ->
+     d_sub_sized E (typ_all S1) T1 (S n)
+ | d__subs__intersection1 : forall (E:denv) (S1 T1 T2:typ) (n1 n2:nat),
      d_sub_sized E S1 T1 n1 ->
      d_sub_sized E S1 T2 n2 ->
-     d_sub_sized E S1 (dtyp_intersection T1 T2) (S (n1 + n2))
- | d__subs__intersection2 : forall (E:denv) (S1 S2 T:dtyp) (n:nat),
+     d_sub_sized E S1 (typ_intersection T1 T2) (S (n1 + n2))
+ | d__subs__intersection2 : forall (E:denv) (S1 S2 T:typ) (n:nat),
      d_sub_sized E S1 T n ->
      dwf_typ E S2 ->
-     d_sub_sized E (dtyp_intersection S1 S2) T (S n)
- | d__subs__intersection3 : forall (E:denv) (S1 S2 T:dtyp) (n:nat),
+     d_sub_sized E (typ_intersection S1 S2) T (S n)
+ | d__subs__intersection3 : forall (E:denv) (S1 S2 T:typ) (n:nat),
      d_sub_sized E S2 T n ->
      dwf_typ E S1 ->
-     d_sub_sized E (dtyp_intersection S1 S2) T (S n)
- | d__subs__union1 : forall (E:denv) (S1 T1 T2:dtyp) (n:nat),
+     d_sub_sized E (typ_intersection S1 S2) T (S n)
+ | d__subs__union1 : forall (E:denv) (S1 T1 T2:typ) (n:nat),
      d_sub_sized E S1 T1 n ->
      dwf_typ E T2 ->
-     d_sub_sized E S1 (dtyp_union T1 T2) (S n)
- | d__subs__union2 : forall (E:denv) (S1 T1 T2:dtyp) (n:nat),
+     d_sub_sized E S1 (typ_union T1 T2) (S n)
+ | d__subs__union2 : forall (E:denv) (S1 T1 T2:typ) (n:nat),
      d_sub_sized E S1 T2 n ->
      dwf_typ E T1 ->
-     d_sub_sized E S1 (dtyp_union T1 T2) (S n)
- | d__subs__union3 : forall (E:denv) (S1 S2 T:dtyp) (n1 n2:nat),
+     d_sub_sized E S1 (typ_union T1 T2) (S n)
+ | d__subs__union3 : forall (E:denv) (S1 S2 T:typ) (n1 n2:nat),
      d_sub_sized E S1 T n1 ->
      d_sub_sized E S2 T n2 ->
-     d_sub_sized E (dtyp_union S1 S2) T (S (n1 + n2)).
+     d_sub_sized E (typ_union S1 S2) T (S (n1 + n2)).
 
 Notation "E ⊢ S1 <: T1 | n" :=
   (d_sub_sized E S1 T1 n)
@@ -888,8 +885,8 @@ Hint Constructors d_sub_sized : sub.
 Lemma d_sub_size_rename_stvar : forall E F SX SY A B n,
     F ++ SX ~ ▪ ++ E ⊢ A <: B | n ->
       SY ∉ (dom E `union` dom F) ->
-      (map (d_subst_stv_in_binding (dtyp_svar SY) SX) F) ++ SY ~ ▪ ++ E ⊢
-        {dtyp_svar SY /ₛᵈ SX} A <: {dtyp_svar SY /ₛᵈ SX} B | n.
+      (map (d_subst_stv_in_binding (typ_svar SY) SX) F) ++ SY ~ ▪ ++ E ⊢
+        {typ_svar SY /ₛᵈ SX} A <: {typ_svar SY /ₛᵈ SX} B | n.
 Proof with (simpl in *; eauto using d_wf_env_subst_tvar_typ with sub).
   intros * HS HN.
   case_eq (SY == SX); intros.
@@ -926,7 +923,7 @@ Proof with (simpl in *; eauto using d_wf_env_subst_tvar_typ with sub).
     solve_notin. inverts* H0.
     forwards* [?|?]: binds_app_1 H3.
     2: { forwards* [(?&?)|?]: binds_cons_1 H0. try solve_by_invert. }
-    forwards* : binds_map_2 (d_subst_stv_in_binding (dtyp_svar SY) SX) H0.
+    forwards* : binds_map_2 (d_subst_stv_in_binding (typ_svar SY) SX) H0.
   - case_if; subst...
     + econstructor.
       applys* d_wf_env_rename_stvar...
@@ -936,19 +933,19 @@ Proof with (simpl in *; eauto using d_wf_env_subst_tvar_typ with sub).
       forwards: d_wf_typ_rename_stvar SY H0...
       case_if in H1...
   - pick fresh SZ and apply d__subs__all. inst_cofinites_with SZ.
-    + rewrite d_subst_stv_in_dtyp_open_comm...
-      applys~ fstv_sins_dtyp_subst_stv_s.
-    + rewrite d_subst_stv_in_dtyp_open_comm...
-      applys~ fstv_sins_dtyp_subst_stv_s.
+    + rewrite d_subst_stv_in_typ_open_comm...
+      applys~ fstv_sins_typ_subst_stv_s.
+    + rewrite d_subst_stv_in_typ_open_comm...
+      applys~ fstv_sins_typ_subst_stv_s.
     + forwards~: H2 SZ E ((SZ, ▪) :: F)...
-      repeat rewrite d_subst_stv_in_dtyp_open_comm...
+      repeat rewrite d_subst_stv_in_typ_open_comm...
   - pick fresh SZ and apply d__subs__alll. 6: apply H4. all: auto...
-    + rewrite d_subst_stv_in_dtyp_open_comm...
-      applys fstv_sins_dtyp_subst_stv...
-    + replace T2 with ({dtyp_svar SY /ₛᵈ SX} T2)...
+    + rewrite d_subst_stv_in_typ_open_comm...
+      applys fstv_sins_typ_subst_stv...
+    + replace T2 with ({typ_svar SY /ₛᵈ SX} T2)...
       forwards: d_wf_typ_rename_stvar SY H3...
     + forwards: IHHS...
-      rewrite d_subst_stv_in_dtyp_open_comm...
+      rewrite d_subst_stv_in_typ_open_comm...
       applys* d_mono_notin_stvar.
   - applys d__subs__intersection2; forwards: IHHS...
     forwards: d_wf_typ_rename_stvar SY H...
@@ -962,16 +959,16 @@ Proof with (simpl in *; eauto using d_wf_env_subst_tvar_typ with sub).
 Qed.
 
 Corollary d_sub_size_rename : forall n X Y D E A B,
-    X `notin`  (fstv_in_dtyp A `union` fstv_in_dtyp B) ->
+    X `notin`  (fstv_in_typ A `union` fstv_in_typ B) ->
     Y `notin` ((dom D) `union` (dom E)) ->
-    D ++ X ~ ▪ ++ E ⊢ A ^^ᵈ dtyp_svar X <: B ^^ᵈ dtyp_svar X | n ->
-    map (d_subst_stv_in_binding (dtyp_svar Y) X) D ++ Y ~ ▪ ++ E ⊢ A ^^ᵈ dtyp_svar Y <: B ^^ᵈ dtyp_svar Y | n.
+    D ++ X ~ ▪ ++ E ⊢ A ^^ᵈ typ_svar X <: B ^^ᵈ typ_svar X | n ->
+    map (d_subst_stv_in_binding (typ_svar Y) X) D ++ Y ~ ▪ ++ E ⊢ A ^^ᵈ typ_svar Y <: B ^^ᵈ typ_svar Y | n.
 Proof with eauto.
   intros.
   forwards: d_sub_size_rename_stvar Y H1. solve_notin.
-  rewrite 2 d_subst_stv_in_dtyp_open_dtyp_wrt_dtyp in H2...
+  rewrite 2 d_subst_stv_in_typ_open_typ_wrt_typ in H2...
   simpl in H2. case_if.
-  rewrite 2 d_subst_stv_in_dtyp_fresh_eq in H2...
+  rewrite 2 d_subst_stv_in_typ_fresh_eq in H2...
 Qed.
 
 Lemma d_sub_size_complete : forall E T1 T2,
@@ -983,7 +980,7 @@ Proof with eauto with sub.
   - pick fresh X.
     destruct (H2 X) as [n]. solve_notin.
     exists (S n).
-    eapply d__subs__all with (L:=L `union` fstv_in_dtyp S1 `union` fstv_in_dtyp S1 `union` (dom E)); intros; eauto.
+    eapply d__subs__all with (L:=L `union` fstv_in_typ S1 `union` fstv_in_typ S1 `union` (dom E)); intros; eauto.
     + rewrite_env (nil ++ SX ~ ▪ ++ E). rewrite_env (nil ++ X ~ ▪ ++ E) in H3.
       applys d_sub_size_rename H3; solve_notin.
   - destruct IHd_sub as [n]. eauto...
@@ -1063,7 +1060,7 @@ Hint Extern 1 (?x > ?y) => lia : trans.
 
 
 Lemma d_sub_size_union_inv: forall E S1 S2 T1 n,
-  E ⊢ (dtyp_union S1 S2) <: T1 | n -> E ⊢ S1 <: T1 | n /\ E ⊢ S2 <: T1 | n.
+  E ⊢ (typ_union S1 S2) <: T1 | n -> E ⊢ S1 <: T1 | n /\ E ⊢ S2 <: T1 | n.
 Proof with auto with trans.
   intros.
   dependent induction H.
@@ -1093,28 +1090,28 @@ Proof.
   apply d_sub_size_complete in H. auto.
 Qed.
 
-Inductive d_ord : dtyp -> Prop :=
-| d__ord__tvar : forall X, d_ord (dtyp_var_f X)
-| d__ord__stvar : forall SX, d_ord (dtyp_svar SX)
-| d__ord__bot : d_ord dtyp_bot
-| d__ord__top : d_ord dtyp_top
-| d__ord__unit : d_ord dtyp_unit
+Inductive d_ord : typ -> Prop :=
+| d__ord__tvar : forall X, d_ord (typ_var_f X)
+| d__ord__stvar : forall SX, d_ord (typ_svar SX)
+| d__ord__bot : d_ord typ_bot
+| d__ord__top : d_ord typ_top
+| d__ord__unit : d_ord typ_unit
 | d__ord__arr : forall T1 T2,
-    d_ord (dtyp_arrow T1 T2)
+    d_ord (typ_arrow T1 T2)
 | d__ord__all : forall T,
-    d_ord (dtyp_all T)
+    d_ord (typ_all T)
 .
 
-Inductive d_wft_ord : dtyp -> Prop :=
+Inductive d_wft_ord : typ -> Prop :=
 | d__wftord__base : forall T, d_ord T -> d_wft_ord T
 | d__wftord__intersection: forall T1 T2,
     d_wft_ord T1 ->
     d_wft_ord T2 ->
-    d_wft_ord (dtyp_intersection T1 T2)
+    d_wft_ord (typ_intersection T1 T2)
 | d__wftord__union: forall T1 T2,
     d_wft_ord T1 ->
     d_wft_ord T2 ->
-    d_wft_ord (dtyp_union T1 T2)
+    d_wft_ord (typ_union T1 T2)
 .
 
 Hint Constructors d_ord : wf.
@@ -1128,7 +1125,7 @@ Qed.
 
 Theorem d_sub_mono_bot_false : forall E T1,
   dmono_typ T1 ->
-  E ⊢ T1 <: dtyp_bot ->
+  E ⊢ T1 <: typ_bot ->
   False.
 Proof.
   intros. induction H; try solve [(dependent destruction H0); auto].
@@ -1139,7 +1136,7 @@ Qed.
 Theorem d_sub_open_mono_bot_false: forall n1 n2 E S1 T1 L,
     d_typ_order (T1 ^^ᵈ S1) < n1 ->
     d_typ_size (T1 ^^ᵈ S1) < n2 ->
-    E ⊢ T1 ^^ᵈ S1 <: dtyp_bot ->
+    E ⊢ T1 ^^ᵈ S1 <: typ_bot ->
     (forall X, X `notin` L -> ds_in X (T1 ^ᵈ X)) ->
     dmono_typ S1 ->
     False.
@@ -1152,47 +1149,47 @@ Proof.
       * destruct T1; simpl in *; try solve [inversion Heq].
         -- inst_cofinites_by L. inversion H3.
         -- destruct n.
-            ++ unfold open_dtyp_wrt_dtyp in Heq. simpl in *.
+            ++ unfold open_typ_wrt_typ in Heq. simpl in *.
                 subst. inversion H4.
-            ++ unfold open_dtyp_wrt_dtyp in Heq. simpl in *.
+            ++ unfold open_typ_wrt_typ in Heq. simpl in *.
                 inversion Heq.
       * destruct T1; simpl in *; try solve [ inversion Heq].
         -- destruct n.
-            ++ unfold open_dtyp_wrt_dtyp in Heq. simpl in *.
+            ++ unfold open_typ_wrt_typ in Heq. simpl in *.
                 subst. inversion H9.
-            ++ unfold open_dtyp_wrt_dtyp in Heq. simpl in *.
+            ++ unfold open_typ_wrt_typ in Heq. simpl in *.
                 inversion Heq.
         -- inversion Heq. subst. eapply IHn1; eauto.
            rewrite d_open_mono_same_order; auto. lia.
       * destruct T1; simpl in *; try solve [inversion Heq].
         -- destruct n.
-           ++ unfold open_dtyp_wrt_dtyp in Heq. simpl in Heq.
+           ++ unfold open_typ_wrt_typ in Heq. simpl in Heq.
               subst. dependent destruction H4.
               eapply d_sub_mono_bot_false with (T1:=S0); eauto.
            ++ inversion Heq.
         -- inversion Heq. subst. eapply IHn2 with (L:=L); eauto.
-           ++ unfold open_dtyp_wrt_dtyp. lia.
-           ++ unfold open_dtyp_wrt_dtyp. lia.
+           ++ unfold open_typ_wrt_typ. lia.
+           ++ unfold open_typ_wrt_typ. lia.
            ++ intros. inst_cofinites_with X. dependent destruction H3; auto.
       * destruct T1; simpl in *; try solve [inversion Heq].
         -- destruct n.
-           ++ unfold open_dtyp_wrt_dtyp in Heq. simpl in Heq.
+           ++ unfold open_typ_wrt_typ in Heq. simpl in Heq.
               subst. dependent destruction H4.
               eapply d_sub_mono_bot_false with (T1:=S2); eauto.
            ++ inversion Heq.
         -- inversion Heq. subst. eapply IHn2 with (L:=L); eauto.
-           ++ unfold open_dtyp_wrt_dtyp. lia.
-           ++ unfold open_dtyp_wrt_dtyp. lia.
+           ++ unfold open_typ_wrt_typ. lia.
+           ++ unfold open_typ_wrt_typ. lia.
            ++ intros. inst_cofinites_with X. dependent destruction H3; auto.
       * destruct T1; simpl in *; try solve [inversion Heq].
         -- destruct n.
-           ++ unfold open_dtyp_wrt_dtyp in Heq. simpl in Heq.
+           ++ unfold open_typ_wrt_typ in Heq. simpl in Heq.
               subst. dependent destruction H3.
               eapply d_sub_mono_bot_false with (T1:=S0); eauto.
            ++ inversion Heq.
         -- inversion Heq. subst. eapply IHn2 with (L:=L); eauto.
-           ++ unfold open_dtyp_wrt_dtyp. lia.
-           ++ unfold open_dtyp_wrt_dtyp. lia.
+           ++ unfold open_typ_wrt_typ. lia.
+           ++ unfold open_typ_wrt_typ. lia.
            ++ intros. inst_cofinites_with X. dependent destruction H2; auto.
 Qed.
 
@@ -1244,8 +1241,8 @@ Ltac solve_trans_forall_B_union_impl T1 T2:=
 Ltac solve_trans_forall_B_iu :=
   match goal with
    | H : ?E ⊢ ?T <: ?C | ?n |- ?E ⊢ ?B <: ?C => match C with
-      | dtyp_intersection ?C1 ?C2 => dependent destruction H; auto with trans; solve_trans_forall_B_intersection_impl C1 C2
-      | dtyp_union ?C1 ?C2 => dependent destruction H; auto with trans; solve_trans_forall_B_union_impl C1 C2
+      | typ_intersection ?C1 ?C2 => dependent destruction H; auto with trans; solve_trans_forall_B_intersection_impl C1 C2
+      | typ_union ?C1 ?C2 => dependent destruction H; auto with trans; solve_trans_forall_B_union_impl C1 C2
       | _ => idtac
    end
   end.
@@ -1254,11 +1251,11 @@ Ltac solve_trans_forall_B_C :=
    match goal with
    | H : ?E ⊢ ?T <: ?C | ?n |- ?E ⊢ ?B <: ?C => match T with
       (* the following case of B is impossible. solve them separately *)
-      | dtyp_bot => idtac
-      | dtyp_svar _ => idtac
-      | dtyp_all _ => idtac
-      | dtyp_union _ _ => idtac
-      | dtyp_intersection _ _ => idtac
+      | typ_bot => idtac
+      | typ_svar _ => idtac
+      | typ_all _ => idtac
+      | typ_union _ _ => idtac
+      | typ_intersection _ _ => idtac
       (* solve the remaining case *)
       | _ => let H1 := fresh H in
              let Hwft1 := fresh "Hwft" in
@@ -1270,8 +1267,8 @@ Ltac solve_trans_forall_B_C :=
 
 Ltac ord_inv :=
     match goal with
-    | H : d_ord (dtyp_intersection _ _) |- _ => inversion H
-    | H : d_ord (dtyp_union _ _)|- _ => inversion H
+    | H : d_ord (typ_intersection _ _) |- _ => inversion H
+    | H : d_ord (typ_union _ _)|- _ => inversion H
    end.
 
 
@@ -1287,26 +1284,26 @@ Proof with auto with trans.
   - dependent destruction Hsub1...
     + dependent destruction Hsub2...
       * econstructor.
-        eapply IHn_dsub_size with (S1:=dtyp_top) (n1:=n2); eauto...
-        eapply IHn_dsub_size with (S1:=dtyp_top) (n1:=n1); eauto...
+        eapply IHn_dsub_size with (S1:=typ_top) (n1:=n2); eauto...
+        eapply IHn_dsub_size with (S1:=typ_top) (n1:=n1); eauto...
       * simpl in H. eapply d_sub_union1.
-        eapply IHn_dsub_size with (S1:=dtyp_top) (n1:=n); eauto...
+        eapply IHn_dsub_size with (S1:=typ_top) (n1:=n); eauto...
         auto.
       * simpl in H. eapply d_sub_union2.
-        eapply IHn_dsub_size with (S1:=dtyp_top) (n1:=n); eauto...
+        eapply IHn_dsub_size with (S1:=typ_top) (n1:=n); eauto...
         auto.
     + apply d_sub_size_sound in Hsub2.
       apply d_sub_dwft in Hsub2; auto.
       eapply d_sub_bot; intuition.
     + dependent destruction Hsub2...
       * econstructor.
-        eapply IHn_dsub_size with (S1:=dtyp_unit) (n1:=n2); eauto...
-        eapply IHn_dsub_size with (S1:=dtyp_unit) (n1:=n1); eauto...
+        eapply IHn_dsub_size with (S1:=typ_unit) (n1:=n2); eauto...
+        eapply IHn_dsub_size with (S1:=typ_unit) (n1:=n1); eauto...
       * simpl in H. eapply d_sub_union1.
-        eapply IHn_dsub_size with (S1:=dtyp_unit) (n1:=n); eauto...
+        eapply IHn_dsub_size with (S1:=typ_unit) (n1:=n); eauto...
         auto.
       * simpl in H. eapply d_sub_union2.
-        eapply IHn_dsub_size with (S1:=dtyp_unit) (n1:=n); eauto...
+        eapply IHn_dsub_size with (S1:=typ_unit) (n1:=n); eauto...
         auto.
     + dependent destruction Hsub2...
       * econstructor.
@@ -1320,13 +1317,13 @@ Proof with auto with trans.
         auto.
     + dependent destruction Hsub2...
       * econstructor.
-        eapply IHn_dsub_size with (S1:=dtyp_svar SX) (n1:=n2); eauto...
-        eapply IHn_dsub_size with (S1:=dtyp_svar SX) (n1:=n1); eauto...
+        eapply IHn_dsub_size with (S1:=typ_svar SX) (n1:=n2); eauto...
+        eapply IHn_dsub_size with (S1:=typ_svar SX) (n1:=n1); eauto...
       * simpl in H. eapply d_sub_union1.
-        eapply IHn_dsub_size with (S1:=dtyp_svar SX) (n1:=n); eauto...
+        eapply IHn_dsub_size with (S1:=typ_svar SX) (n1:=n); eauto...
         auto.
       * simpl in H. eapply d_sub_union2.
-        eapply IHn_dsub_size with (S1:=dtyp_svar SX) (n1:=n); eauto...
+        eapply IHn_dsub_size with (S1:=typ_svar SX) (n1:=n); eauto...
         auto.
     + simpl in *. dependent destruction Hsub2...
       * econstructor... apply d_sub_size_sound in Hsub1_1. apply d_sub_size_sound in Hsub1_2.
@@ -1335,13 +1332,13 @@ Proof with auto with trans.
         eapply IHn_dsub_size with (S1:=T0); eauto...
         eapply IHn_dsub_size with (S1:=T2); eauto...
       * econstructor.
-        eapply IHn_dsub_size with (S1:=dtyp_arrow T0 T2) (n1:=S(n1+n0)); eauto...
-        eapply IHn_dsub_size with (S1:=dtyp_arrow T0 T2) (n1:=S(n1+n0)); eauto...
+        eapply IHn_dsub_size with (S1:=typ_arrow T0 T2) (n1:=S(n1+n0)); eauto...
+        eapply IHn_dsub_size with (S1:=typ_arrow T0 T2) (n1:=S(n1+n0)); eauto...
       * apply d_sub_union1.
-        eapply IHn_dsub_size with (S1:=dtyp_arrow T0 T2) (n1:=S(n1+n0)); eauto...
+        eapply IHn_dsub_size with (S1:=typ_arrow T0 T2) (n1:=S(n1+n0)); eauto...
         auto.
       * apply d_sub_union2.
-        eapply IHn_dsub_size with (S1:=dtyp_arrow T0 T2) (n1:=S(n1+n0)); eauto...
+        eapply IHn_dsub_size with (S1:=typ_arrow T0 T2) (n1:=S(n1+n0)); eauto...
         auto.
     + simpl in *. dependent destruction Hsub2...
       * econstructor...
@@ -1353,12 +1350,12 @@ Proof with auto with trans.
            rewrite_env (nil ++ SY ~ ▪ ++ E) in H4.
            rewrite_env (nil ++ SY ~ ▪ ++ E) in H5.
            forwards: d_wf_typ_subst_stvar_tvar H5.
-           simpl in H6. rewrite d_subst_stv_in_dtyp_open_dtyp_wrt_dtyp in H6.
-           simpl in H6. case_if. rewrite* d_subst_stv_in_dtyp_fresh_eq in H6.
+           simpl in H6. rewrite d_subst_stv_in_typ_open_typ_wrt_typ in H6.
+           simpl in H6. case_if. rewrite* d_subst_stv_in_typ_fresh_eq in H6.
            solve_notin. now eauto.
       * eapply d_sub_all with (L:=L `union` L0 `union` dom E); auto.
         intros. inst_cofinites_with SX.
-        eapply IHn_d_typ_order with (S1:= T0 ^^ᵈ dtyp_svar SX); eauto...
+        eapply IHn_d_typ_order with (S1:= T0 ^^ᵈ typ_svar SX); eauto...
         -- simpl in *. rewrite d_open_svar_same_order.
            assert ((d_typ_order T0) < n_d_typ_order) by lia. (* lia strangely fails if proving directly *)
            auto.
@@ -1373,22 +1370,22 @@ Proof with auto with trans.
         eapply IHn_d_typ_order with (S1:=T0 ^^ᵈ T2) (n1:=n'); eauto...
         rewrite d_open_mono_same_order; auto. now lia.
         simpl in Hsub. auto. simpl.
-        rewrite 2 d_subst_stv_in_dtyp_open_dtyp_wrt_dtyp in Hsub... simpl in Hsub.
+        rewrite 2 d_subst_stv_in_typ_open_typ_wrt_typ in Hsub... simpl in Hsub.
         unfold eq_dec in Hsub. destruct (EqDec_eq_of_X SX SX) in Hsub.
-        rewrite (d_subst_stv_in_dtyp_fresh_eq S1) in Hsub...
-        rewrite (d_subst_stv_in_dtyp_fresh_eq T0) in Hsub...
+        rewrite (d_subst_stv_in_typ_fresh_eq S1) in Hsub...
+        rewrite (d_subst_stv_in_typ_fresh_eq T0) in Hsub...
         contradiction.
       * eapply d_sub_intersection1.
-        -- eapply IHn_dsub_size with (S1:=dtyp_all T0) (n1:=S n) (n2:=n1); eauto...
+        -- eapply IHn_dsub_size with (S1:=typ_all T0) (n1:=S n) (n2:=n1); eauto...
            econstructor; eauto.
-        -- eapply IHn_dsub_size with (S1:=dtyp_all T0) (n1:=S n) (n2:=n2); eauto...
+        -- eapply IHn_dsub_size with (S1:=typ_all T0) (n1:=S n) (n2:=n2); eauto...
            econstructor; eauto.
       * eapply d_sub_union1.
-        -- eapply IHn_dsub_size with (S1:=dtyp_all T0) (n1:=S n) (n2:=n0); eauto...
+        -- eapply IHn_dsub_size with (S1:=typ_all T0) (n1:=S n) (n2:=n0); eauto...
            econstructor; eauto.
         -- auto.
       * eapply d_sub_union2.
-        -- eapply IHn_dsub_size with (S1:=dtyp_all T0) (n1:=S n) (n2:=n0); eauto...
+        -- eapply IHn_dsub_size with (S1:=typ_all T0) (n1:=S n) (n2:=n0); eauto...
            econstructor; eauto.
         -- auto.
     + simpl in *. assert (E ⊢ T0) as Hwft0 by applys* d_sub_dwft_sized_1.
@@ -1433,7 +1430,7 @@ Proof with auto with trans.
            forwards*: d_wf_typ_open_stvar_subst_mono HW.
         -- assert (E ⊢ T1) by applys* d_sub_dwft_sized_1. assert (E ⊢ T4) by applys* d_sub_dwft_sized_2.
           eapply d_sub_alll with (T2:=T2); eauto...
-          eapply IHn_dsub_size with (S1:=dtyp_arrow T0 T3) (n2:=S(n1+n2)); eauto...
+          eapply IHn_dsub_size with (S1:=typ_arrow T0 T3) (n2:=S(n1+n2)); eauto...
       * inversion H.
       * inversion H1.
       * inversion H0.
@@ -1441,14 +1438,14 @@ Proof with auto with trans.
       * econstructor... apply d_sub_size_sound in Hsub1_1. apply d_sub_dwft in Hsub1_1.
         intuition.
       * econstructor.
-        eapply IHn_dsub_size with (S1:=dtyp_intersection T0 T2) (n1:=S(n1+n0)); eauto...
-        eapply IHn_dsub_size with (S1:=dtyp_intersection T0 T2) (n1:=S(n1+n0)); eauto...
+        eapply IHn_dsub_size with (S1:=typ_intersection T0 T2) (n1:=S(n1+n0)); eauto...
+        eapply IHn_dsub_size with (S1:=typ_intersection T0 T2) (n1:=S(n1+n0)); eauto...
       * eapply IHn_dsub_size with (S1:=T0); eauto...
       * eapply IHn_dsub_size with (S1:=T2); eauto...
       * apply d_sub_union1...
-        eapply IHn_dsub_size with (S1:=dtyp_intersection T0 T2) (n1:=S(n1+n0)); eauto...
+        eapply IHn_dsub_size with (S1:=typ_intersection T0 T2) (n1:=S(n1+n0)); eauto...
       * apply d_sub_union2...
-        eapply IHn_dsub_size with (S1:=dtyp_intersection T0 T2) (n1:=S(n1+n0)); eauto...
+        eapply IHn_dsub_size with (S1:=typ_intersection T0 T2) (n1:=S(n1+n0)); eauto...
     + simpl in H. apply d_sub_intersection2...
       * eapply IHn_dsub_size with (S1:=T) (n1:=n); eauto...
     + simpl in H. apply d_sub_intersection3...
